theories/prelude/elpi/derive/finset.v
@@ -16,15 +16,15 @@ From bedrock.prelude.elpi Require Import prelude derive.plugins.
  ***************************************************)
 Elpi Db derive.finset.db lp:{{
   namespace derive.finset {
-    pred mk-finite-prelim i:string.
-    mk-finite-prelim TypeName :- std.do! [
-      coq.locate TypeName GR,
+    pred mk-finite-prelim i:string, i:gref.
+    mk-finite-prelim TypeName TyGR :- std.do! [
+      #line 21 "derive.v"
       %TODO: I'd like to be able to do a transparent ascription here, but
       %it doesn't seem like coq-elpi supports this (the following gives opaque ascription):
       %coq.locate-module-type "simple_finite_bitmask_type_intf" MTP,
       coq.env.begin-module TypeName none,
 
-      coq.env.add-const "t" (global GR) _ @transparent! C,
+      coq.env.add-const "t" (global TyGR) _ @transparent! C,
       Ty = global (const C),
 
       %TODO: these names are couplings, so centralize the calculation of instance names
@@ -42,21 +42,22 @@ Elpi Db derive.finset.db lp:{{
       @global! => coq.TC.declare-instance (const Cfin) 0,
     ].
 
-    pred mk-simple-finite i:string.
-    mk-simple-finite TypeName :- std.do! [
-      mk-finite-prelim TypeName,
+    pred mk-simple-finite i:string, i:gref.
+    mk-simple-finite TypeName TyGR :- std.do! [
+      derive.if-verbose (coq.say "[derive.finset][mk-simple-finite]" TypeName),
+      mk-finite-prelim TypeName TyGR,
       coq.env.include-module-type {coq.locate-module-type "finite_type_mixin"} coq.inline.default,
       coq.env.end-module MP_,
     ].
 
-    pred mk-finite i:string, i:string.
-    mk-finite TypeName ToN :- std.do! [
-      mk-finite-prelim TypeName,
+    pred mk-finite i:string, i:gref, i:term.
+    mk-finite TypeName TyGR ToN :- std.do! [
+      derive.if-verbose (coq.say "[derive.finset][mk-finite]" TypeName),
+      mk-finite-prelim TypeName TyGR,
 
       coq.locate "t" GRTy,
       Ty is global GRTy,
-      coq.locate ToN GRtoN,
-      coq.env.add-const "to_N" (global GRtoN) {{ lp:Ty -> N }} @transparent! CtoN_,
+      coq.env.add-const "to_N" ToN {{ lp:Ty -> N }} @transparent! CtoN_,
 
       coq.env.include-module-type {coq.locate-module-type "finite_encoded_type_mixin"} coq.inline.default,
       coq.env.end-module MP_,
@@ -64,13 +65,35 @@ Elpi Db derive.finset.db lp:{{
   }
 }}.
 
+Elpi Accumulate derive lp:{{
+  namespace derive.finset {
+    pred to-N i:term, o:term.
+    :name "to-N.fail"
+    to-N T F :- std.do! [
+      Lem = {{ @ToN lp:T lp:F }},
+      derive.if-verbose (coq.say "[derive.finset][to-N]" Lem),
+      std.assert-ok! (coq.typecheck {{ lp:Bo : lp:Lem }} _) "typechecking a [ToN] instance failed",
+      coq.ltac.collect-goals Bo [SealedGoal] [],
+      coq.ltac.open (coq.ltac.call "typeclasses_eauto" []) SealedGoal [],
+      derive.if-verbose (coq.say "[derive.finset][to-N]" T Lem),
+      %Memoize the result:
+      coq.elpi.accumulate library "derive.finset.db" (clause _ (before "to-N.fail") (to-N T F)),
+    ].
+  }
+}}.
+
+(*We must export this tactic to [[ #[only(finset)] derive ]] use sites.*)
+Ltac typeclasses_eauto := typeclasses eauto.
+
 Elpi Accumulate derive Db derive.finset.db.
 Elpi Accumulate derive lp:{{
   namespace derive.finset {
     pred main i:gref, i:string, o:list prop.
     main TyGR Prefix Clauses :- std.do! [
-        remove-final-underscore Prefix Variant,
-      derive.finset.mk-simple-finite Variant,
+      remove-final-underscore Prefix Variant,
+      if (derive.finset.to-N (global TyGR) ToN)
+        (derive.finset.mk-finite Variant TyGR ToN)
+        (derive.finset.mk-simple-finite Variant TyGR),
       Clauses = [finset-done TyGR],
       std.forall Clauses (x\
         coq.elpi.accumulate _ "derive.finbitset.db" (clause _ _ x)
